more clean up

theories2/astCast.v
@@ -25,7 +25,7 @@ with term : Type :=
 | Cast (s : term) (l : term)
 
 | Lump (terms : list term) (t : term) (* TODO: cast just a singleton lump? *)
-| assertEq (l r t : term) (p : path) (* TODO attach type assertion? *)
+| assertEq (l r t : term) (p : path) (* TODO attach or remove type assertion? *)
 | Arg (l : term)
 | Bod (a :term) (l : term)
 (* | Ap (a :term) (l : term) *)
@@ -38,10 +38,6 @@ Axiom Eq : (list term) -> term -> term -> term -> Prop.
 
 (* endpoints *)
 Reserved Notation "[ Gamma |- s ~= a :- A ]".
-
-Axiom LumpOk : (list term) -> (term) -> Prop.
-
-(* TODO: merge with above *)
 
 
 Inductive has_enpoint : list term -> term -> term -> term -> Prop :=
@@ -141,133 +137,13 @@ with Connected : (list term) -> (list term) -> Prop :=
   has_enpoint ctx a a' A' ->
   has_enpoint ctx b b' B' ->
   Connected ctx (cons b rest)
+with LumpOk : (list term) -> (term) -> Prop :=
+
 
 .
 
 Definition ty (ctx : list term) (a : term) (A : term) := 
   has_enpoint ctx a a A.
 
-Axiom extract_ty : term -> term.
-
-Axiom Union : term -> term ->  term.
-
-Inductive step : term -> term -> Prop :=
-  (* beta reductions - app *)
-  (* | step_beta b a :
-      value a ->
-      step (App (Fun b) a) (b.[Fun b,  a /]) *)
-  
-  | step_cast_beta b a l :
-  (* value a -> *)
-  step
-    (App (Cast b l) a)
-    (Cast (App b (Cast a (Arg l))) (Bod a l))
-
-  | step_Lump_beta a ls L :
-  (* value a -> *)
-  step
-    (App (Lump ls L) a)
-    (Lump (map (fun x => App x a) ls) (Bod a L))
-
-  | step_assert_beta b c t p a :
-  (* value a -> *)
-  step
-    (App (assertEq b c t p) a)
-    (assertEq (App b a) (App c a) (Bod a t) (AObs a p))
-    (* other reductions *)
-  | step_cast_collapse a l l' :
-    (* value ... -> *)
-    step
-      (Cast (Cast a l) l')
-      (Cast a (Union l l'))
-(* lump *)
-  | step_Lump l l' L L' :
-  (* value... -> *)
-  (* TODO this does not only need to happen to the first element *)
-  step
-    (Lump (cons (Lump l L) l') L')
-    (Lump (l ++ l') (Union L L' ))
-
-  | step_Lump_cast a l' L L' :
-    (* value ... -> *)
-    (* TODO this does not only need to happen to the first element *)
-    step
-      (Lump (cons (Cast a L) l') L')
-      (Lump (cons a l') (Union L L' ))
-(* assert *)
-
-| step_Assert_castL a b L L' o :
-  step
-  (assertEq (Cast a L) b L' o)
-  (assertEq a b (Union L L') o)
-  
-
-  | step_Assert_castR a b L L' o :
-  step
-  (assertEq a (Cast b L) L' o)
-  (assertEq a b (Union L L') o)
-
-(* other reductions *)
-
-(* Arg *)
-  | step_Arg A B :
-  step
-    (Arg (Pi A B))
-    A
-
-  | step_Arg_Assert A B A' B' p:
-  step
-    (Arg (assertEq (Pi A B) (Pi A' B') TT p))
-    (assertEq A A' TT (ArgObs p))
-
-  | step_Arg_Lump ls:
-  step
-    (Arg (Lump ls TT))
-    (Lump (map (Arg) ls) TT)
-
-    (* Bod *)
-  (* | step_Bod a A B :
-  step
-    (Bod a (Pi A B))
-    (B.[a/]) *)
-
-  (* | step_Bod_Assert a A B A' B' p:
-  step
-    (Bod a (assertEq (Pi A B) (Pi A' B') TT p))
-    (assertEq (B.[a/]) (B'.[a/]) TT (BodTyObs a p)) *)
-
-  | step_Bod_Lump a ls:
-  step
-    (Bod a (Lump ls TT))
-    (Lump (map (Bod a) ls) TT)
-
-  (* structrural rules *)
-  (* ,,, *)
-.
-
-
-(* Assume Eq is a congruent equivelence that respects step.  And... *)
-(* Axiom Casts_dont_matter ctx a a' L L' A' B : 
-  has_enpoint ctx a a' A ->
-  has_enpoint ctx L A' TT ->
-  has_enpoint ctx L B TT ->
-  LumpOk ctx L ->
-
-  has_enpoint ctx L' A' TT ->
-  has_enpoint ctx L' B TT ->
-  LumpOk ctx L' ->
-
-  Eq ctx (Cast a L) (Cast a L') B. *)
-
-(* Axiom vacCast ctx a a' L L' A' B : 
-  ty ctx a A 
-  Eq ctx a (Cast a (cons A Nil)) A. *)
-
-
-Lemma preservation ctx a a' A a2 : 
-  has_enpoint ctx a a' A -> 
-  step a a2 ->
-  has_enpoint ctx a2 a' A.
-Admitted.
 
 
