theories2/smallstepCast.v
@@ -1,0 +1,136 @@
+
+
+From mathcomp Require Import ssreflect ssrbool eqtype ssrnat seq.
+From Coq Require Import ssrfun.
+Require Import AutosubstSsr ARS Context.
+Require Import Program.Equality.
+
+Set Implicit Arguments.
+Unset Strict Implicit.
+Unset Printing Implicit Defensive.
+
+
+Require Import astCast.
+
+Axiom extract_ty : term -> term.
+
+Axiom Union : term -> term ->  term.
+
+Inductive step : term -> term -> Prop :=
+  (* beta reductions - app *)
+  (* | step_beta b a :
+      value a ->
+      step (App (Fun b) a) (b.[Fun b,  a /]) *)
+  
+  | step_cast_beta b a l :
+  (* value a -> *)
+  step
+    (App (Cast b l) a)
+    (Cast (App b (Cast a (Arg l))) (Bod a l))
+
+  | step_Lump_beta a ls L :
+  (* value a -> *)
+  step
+    (App (Lump ls L) a)
+    (Lump (map (fun x => App x a) ls) (Bod a L))
+
+  | step_assert_beta b c t p a :
+  (* value a -> *)
+  step
+    (App (assertEq b c t p) a)
+    (assertEq (App b a) (App c a) (Bod a t) (AObs a p))
+    (* other reductions *)
+  | step_cast_collapse a l l' :
+    (* value ... -> *)
+    step
+      (Cast (Cast a l) l')
+      (Cast a (Union l l'))
+(* lump *)
+  | step_Lump l l' L L' :
+  (* value... -> *)
+  (* TODO this does not only need to happen to the first element *)
+  step
+    (Lump (cons (Lump l L) l') L')
+    (Lump (l ++ l') (Union L L' ))
+
+  | step_Lump_cast a l' L L' :
+    (* value ... -> *)
+    (* TODO this does not only need to happen to the first element *)
+    step
+      (Lump (cons (Cast a L) l') L')
+      (Lump (cons a l') (Union L L' ))
+(* assert *)
+
+| step_Assert_castL a b L L' o :
+  step
+  (assertEq (Cast a L) b L' o)
+  (assertEq a b (Union L L') o)
+  
+
+  | step_Assert_castR a b L L' o :
+  step
+  (assertEq a (Cast b L) L' o)
+  (assertEq a b (Union L L') o)
+
+(* other reductions *)
+
+(* Arg *)
+  | step_Arg A B :
+  step
+    (Arg (Pi A B))
+    A
+
+  | step_Arg_Assert A B A' B' p:
+  step
+    (Arg (assertEq (Pi A B) (Pi A' B') TT p))
+    (assertEq A A' TT (ArgObs p))
+
+  | step_Arg_Lump ls:
+  step
+    (Arg (Lump ls TT))
+    (Lump (map (Arg) ls) TT)
+
+    (* Bod *)
+  (* | step_Bod a A B :
+  step
+    (Bod a (Pi A B))
+    (B.[a/]) *)
+
+  (* | step_Bod_Assert a A B A' B' p:
+  step
+    (Bod a (assertEq (Pi A B) (Pi A' B') TT p))
+    (assertEq (B.[a/]) (B'.[a/]) TT (BodTyObs a p)) *)
+
+  | step_Bod_Lump a ls:
+  step
+    (Bod a (Lump ls TT))
+    (Lump (map (Bod a) ls) TT)
+
+  (* structrural rules *)
+  (* ,,, *)
+.
+
+
+(* Assume Eq is a congruent equivelence that respects step.  And... *)
+(* Axiom Casts_dont_matter ctx a a' L L' A' B : 
+  has_enpoint ctx a a' A ->
+  has_enpoint ctx L A' TT ->
+  has_enpoint ctx L B TT ->
+  LumpOk ctx L ->
+
+  has_enpoint ctx L' A' TT ->
+  has_enpoint ctx L' B TT ->
+  LumpOk ctx L' ->
+
+  Eq ctx (Cast a L) (Cast a L') B. *)
+
+(* Axiom vacCast ctx a a' L L' A' B : 
+  ty ctx a A 
+  Eq ctx a (Cast a (cons A Nil)) A. *)
+
+
+Lemma preservation ctx a a' A a2 : 
+  has_enpoint ctx a a' A ->   (* why isn't this importerd? *)
+  step a a2 ->
+  has_enpoint ctx a2 a' A.
+Admitted.
